Morph.lean
@@ -1,4 +1,14 @@
+/- Copyright 2024-2025 The Morph Project Authors
+SPDX-License-Identifier: Apache-2.0
+-/
+
 import Morph.Core
 import Morph.Syntax
 import Morph.HIR
 import Morph.MIR
+import Morph.XIR.Types
+import Morph.XIR.Instructions
+import Morph.XIR.CFG
+import Morph.Compiler.HIRToMIR
+import Morph.Compiler.MIRToXIR
+import Morph.Backends
