Morph/Proofs.lean
@@ -1,0 +1,3 @@
+/- Copyright 2024-2025 The Morph Project Authors
+SPDX-License-Identifier: Apache-2.0
+-/
